examples/Query.v
@@ -1,0 +1,89 @@
+Require Import ZArith.
+
+(* Import the SMTCoq-API Library *)
+Require Import SMTCoqApi.
+Require Import SMTCoq.bva.BVList.
+Import BITVECTOR_LIST.
+
+Import ListNotations.
+Import EqNotations.
+
+Definition model1 := model_set_fun default_model 0 [] Sort_Int 5%Z.
+
+Definition query1 :=
+    {|
+      declarations := [];
+      assertions := [
+        Term_Eq (Term_Fun (0, ([], Sort_Int)) []) (Term_Int 5)
+      ]
+    |}.
+
+Goal SAT query1.
+  exists model1. repeat constructor.
+Qed.
+
+Definition query2 :=
+    {|
+      declarations := [];
+      assertions := [
+        Term_Eq (Term_Int 5) (Term_Int 5)
+      ]
+    |}.
+
+Goal valid query2.
+  unfold valid, satisfied_by.
+  intros.
+  repeat constructor.
+Qed.
+
+Definition query3 :=
+    {|
+      declarations := [];
+      assertions := [
+        Term_Eq (Term_Int 2) (Term_Int 5)
+      ]
+    |}.
+
+(* The injection tactic fails for terms like Some (existT _ _ _ ) = Some (existT _ _ _), so we use this lemma instead *)
+Lemma some_injection {A} (x y : A) :
+  Some x = Some y -> x = y.
+Proof. congruence. Qed.
+
+Goal invalid query3.
+  unfold invalid, satisfied_by.
+  intros.
+  exists default_model.
+  inversion 1; subst.
+  match goal with
+  | [ H : term_satisfied_by _ _ |- _ ] => inversion H
+  end.
+  simpl in *.
+  apply some_injection in H0.
+  inversion_sigma; rewrite <- Eqdep_dec.eq_rect_eq_dec in * by exact dec_sort.
+  discriminate.
+Qed.
+
+Example t2 :
+  UNSAT
+    {|
+      declarations := [];
+      assertions := [
+        Term_Eq (Term_Fun (0, ([], Sort_Int)) []) (Term_Int 5);
+        Term_Eq (Term_Fun (0, ([], Sort_Int)) []) (Term_Int 2)
+      ]
+    |}.
+Proof.
+  unfold UNSAT, not, satisfied_by. intros.
+  simpl in *.
+  repeat match goal with
+         | [ H : Forall _ _ |- _ ] => inversion H; subst; clear H
+         end.
+  unfold term_satisfied_by in *.
+  simpl in *.
+  apply some_injection in H1.
+  apply some_injection in H2.
+  inversion_sigma.
+  rewrite <- Eqdep_dec.eq_rect_eq_dec in * by exact dec_sort.
+  rewrite Z.eqb_eq in *.
+  congruence.
+Qed.
